Upd

VRF/Spec_VRF.ml
@@ -1,0 +1,365 @@
+open Prims
+type bytes = FStar_UInt8.t FStar_Seq_Base.seq
+type key = Prims.unit FStar_Endianness.lbytes
+let field: Prims.int = Spec_Curve25519.prime
+let n: Prims.int = Prims.parse_int "32"
+let d: Prims.int =
+  Prims.parse_int
+    "37095705934669439343138083508754565189542113879843219016388785533085940283555"
+type twisted_edward_point = Spec_Ed25519.ext_point
+let scalarMultiplication:
+  twisted_edward_point -> bytes -> Spec_Ed25519.ext_point =
+  fun point  -> fun k1  -> Spec_Ed25519.point_mul k1 point
+let scalarAddition:
+  twisted_edward_point -> twisted_edward_point -> Spec_Ed25519.ext_point =
+  fun p  -> fun q1  -> Spec_Ed25519.point_add p q1
+let isPointOnCurve: twisted_edward_point option -> Prims.bool =
+  fun point  ->
+    if FStar_Option.isNone point
+    then false
+    else
+      (match FStar_Option.get point with
+       | (px,py,pz,pt) ->
+           (Spec_Curve25519.fsub (Spec_Curve25519.fmul px px)
+              (Spec_Curve25519.fmul py py))
+             =
+             (Spec_Curve25519.fadd (Spec_Curve25519.fmul pz pz)
+                (Spec_Curve25519.fmul d (Spec_Curve25519.fmul pt pt))))
+let serializePoint: twisted_edward_point -> Prims.unit Spec_Lib.lbytes =
+  fun point  -> Spec_Ed25519.point_compress point
+let deserializePoint: bytes -> Spec_Ed25519.ext_point option =
+  fun b  -> Spec_Ed25519.point_decompress b
+let _OS2ECP: bytes -> twisted_edward_point option =
+  fun point  -> deserializePoint point
+let _ECP2OS: twisted_edward_point -> bytes =
+  fun gamma  -> serializePoint gamma
+let nat_to_uint8: Prims.int -> FStar_UInt8.t =
+  fun x  ->
+    FStar_UInt8.uint_to_t (FStar_UInt.to_uint_t (Prims.parse_int "8") x)
+let uint8_to_int: FStar_UInt8.t -> Prims.unit FStar_UInt.uint_t =
+  fun x  -> FStar_UInt8.v x
+let rec _helper_I2OSP:
+  Prims.nat -> bytes -> Prims.nat -> FStar_UInt8.t FStar_Seq_Base.seq =
+  fun value  ->
+    fun s  ->
+      fun counter  ->
+        if
+          (counter + (Prims.parse_int "1")) <
+            (FStar_Seq_Base.length
+               (FStar_Seq_Base.upd s counter
+                  (nat_to_uint8 (value mod (Prims.parse_int "256")))))
+        then
+          _helper_I2OSP (value / (Prims.parse_int "256"))
+            (FStar_Seq_Base.upd s counter
+               (nat_to_uint8 (value mod (Prims.parse_int "256"))))
+            (counter + (Prims.parse_int "1"))
+        else
+          FStar_Seq_Base.upd s counter
+            (nat_to_uint8 (value mod (Prims.parse_int "256")))
+let _I2OSP: Prims.nat -> Prims.int -> bytes =
+  fun value  ->
+    fun n1  ->
+      if (Prims.pow2 (FStar_Mul.op_Star n1 (Prims.parse_int "8"))) <= value
+      then
+        FStar_Seq_Base.create n1
+          (FStar_UInt8.uint_to_t (Prims.parse_int "0"))
+      else
+        _helper_I2OSP value
+          (FStar_Seq_Base.create n1
+             (FStar_UInt8.uint_to_t (Prims.parse_int "0")))
+          (Prims.parse_int "0")
+let rec _helper_OS2IP: bytes -> Prims.nat -> Prims.nat -> Prims.nat =
+  fun s  ->
+    fun counter  ->
+      fun number  ->
+        if (counter + (Prims.parse_int "1")) = (FStar_Seq_Base.length s)
+        then
+          number +
+            ((Prims.pow2 (FStar_Mul.op_Star (Prims.parse_int "8") counter)) *
+               (uint8_to_int (FStar_Seq_Base.index s counter)))
+        else
+          _helper_OS2IP s (counter + (Prims.parse_int "1"))
+            (number +
+               ((Prims.pow2 (FStar_Mul.op_Star (Prims.parse_int "8") counter))
+                  * (uint8_to_int (FStar_Seq_Base.index s counter))))
+let _OS2IP: bytes -> Prims.nat =
+  fun s  -> _helper_OS2IP s (Prims.parse_int "0") (Prims.parse_int "0")
+
+let seqConcat s1 s2 = FStar_Seq_Base.append s1 s2
+
+let hash: bytes -> Spec_SHA2_256.bytes =
+  fun input  -> Spec_SHA2_256.hash input
+(*)
+let _ECVRF_decode_proof: bytes -> (twisted_edward_point option* bytes* bytes)
+  =
+  fun pi  ->
+    match FStar_Seq_Properties.split pi n with
+    | (gamma,cs) ->
+        (match FStar_Seq_Properties.split cs n with
+         | (c,s) -> ((_OS2ECP gamma), c, s))
+
+let rec _helper_ECVRF_hash_to_curve:
+  Prims.nat -> Prims.nat -> bytes -> bytes -> twisted_edward_point option =
+  fun ctr  ->
+    fun counter_length  ->
+      fun pk  ->
+        fun input  ->
+          if
+            FStar_Option.isNone
+              (_OS2ECP
+                 (hash
+                    (seqConcat (seqConcat input pk)
+                       (_I2OSP ctr counter_length))))
+          then None
+          else
+            if
+              isPointOnCurve
+                (_OS2ECP
+                   (hash
+                      (seqConcat (seqConcat input pk)
+                         (_I2OSP ctr counter_length))))
+            then
+              _OS2ECP
+                (hash
+                   (seqConcat (seqConcat input pk)
+                      (_I2OSP ctr counter_length)))
+            else
+              if (ctr + (Prims.parse_int "1")) < field
+              then
+                _helper_ECVRF_hash_to_curve (ctr + (Prims.parse_int "1"))
+                  counter_length pk input
+              else None
+let _ECVRF_hash_to_curve:
+  bytes -> twisted_edward_point -> twisted_edward_point option =
+  fun input  ->
+    fun public_key  ->
+      _helper_ECVRF_hash_to_curve (Prims.parse_int "0") (Prims.parse_int "4")
+        (_ECP2OS public_key) input
+let random: Prims.nat -> Prims.nat =
+  Obj.magic (fun max1  -> failwith "Not yet implemented:random")
+let randBytes: Prims.nat -> bytes =
+  fun max1  -> _I2OSP (random max1) (Prims.parse_int "32")
+let _ECVRF_hash_points:
+  twisted_edward_point ->
+    twisted_edward_point ->
+      twisted_edward_point ->
+        twisted_edward_point ->
+          twisted_edward_point -> twisted_edward_point -> Prims.nat
+  =
+  fun generator  ->
+    fun h  ->
+      fun public_key  ->
+        fun gamma  ->
+          fun gk  ->
+            fun hk  ->
+              _OS2IP
+                (fst
+                   (FStar_Seq_Properties.split
+                      (hash
+                         (seqConcat
+                            (seqConcat
+                               (seqConcat
+                                  (seqConcat
+                                     (seqConcat (_ECP2OS generator)
+                                        (_ECP2OS h)) (_ECP2OS public_key))
+                                  (_ECP2OS gamma)) (_ECP2OS gk)) (_ECP2OS hk)))
+                      n))
+let _ECVRF_prove:
+  bytes ->
+    twisted_edward_point -> bytes -> twisted_edward_point -> bytes option
+  =
+  fun input  ->
+    fun public_key  ->
+      fun private_key  ->
+        fun generator  ->
+          if FStar_Option.isNone (_ECVRF_hash_to_curve input public_key)
+          then None
+          else
+            Some
+              (seqConcat
+                 (_ECP2OS
+                    (scalarMultiplication
+                       (FStar_Option.get
+                          (_ECVRF_hash_to_curve input public_key))
+                       private_key))
+                 (seqConcat
+                    (_I2OSP
+                       (_ECVRF_hash_points generator
+                          (FStar_Option.get
+                             (_ECVRF_hash_to_curve input public_key))
+                          public_key
+                          (scalarMultiplication
+                             (FStar_Option.get
+                                (_ECVRF_hash_to_curve input public_key))
+                             private_key)
+                          (scalarMultiplication generator
+                             (_I2OSP (random field) (Prims.parse_int "32")))
+                          (scalarMultiplication
+                             (FStar_Option.get
+                                (_ECVRF_hash_to_curve input public_key))
+                             (_I2OSP (random field) (Prims.parse_int "32"))))
+                       n)
+                    (_I2OSP
+                       (((random field) + field) -
+                          (((_ECVRF_hash_points generator
+                               (FStar_Option.get
+                                  (_ECVRF_hash_to_curve input public_key))
+                               public_key
+                               (scalarMultiplication
+                                  (FStar_Option.get
+                                     (_ECVRF_hash_to_curve input public_key))
+                                  private_key)
+                               (scalarMultiplication generator
+                                  (_I2OSP (random field)
+                                     (Prims.parse_int "32")))
+                               (scalarMultiplication
+                                  (FStar_Option.get
+                                     (_ECVRF_hash_to_curve input public_key))
+                                  (_I2OSP (random field)
+                                     (Prims.parse_int "32"))))
+                              * field)
+                             mod field)) ((Prims.parse_int "2") * n))))
+let _ECVRF_proof2hash: bytes -> FStar_UInt8.t FStar_Seq_Base.seq =
+  fun pi  -> fst (FStar_Seq_Properties.split pi n)
+let _ECVRF_verify:
+  twisted_edward_point ->
+    twisted_edward_point -> bytes -> bytes -> Prims.bool
+  =
+  fun generator  ->
+    fun public_key  ->
+      fun pi  ->
+        fun input  ->
+          match _ECVRF_decode_proof pi with
+          | (gamma,c,s) ->
+              if Prims.op_Negation (isPointOnCurve gamma)
+              then false
+              else
+                if FStar_Option.isNone gamma
+                then false
+                else
+                  if
+                    FStar_Option.isNone
+                      (_ECVRF_hash_to_curve input public_key)
+                  then false
+                  else
+                    (_OS2IP c) =
+                      (_ECVRF_hash_points generator
+                         (FStar_Option.get
+                            (_ECVRF_hash_to_curve input public_key))
+                         public_key (FStar_Option.get gamma)
+                         (scalarAddition (scalarMultiplication public_key c)
+                            (scalarMultiplication generator s))
+                         (scalarAddition
+                            (scalarMultiplication (FStar_Option.get gamma) c)
+                            (scalarMultiplication
+                               (FStar_Option.get
+                                  (_ECVRF_hash_to_curve input public_key)) s)))
+
+*)
+
+let one = Prims.parse_int "1"
+let zero = Prims.parse_int "0"    
+
+
+
+let createTwistedEdwardPoint (a: Prims.int)  (b : Prims.int) (c : Prims.int) (d : Prims.int) : Spec_Ed25519.ext_point  =  
+(a,b,c,d)
+
+let printTwistedEdwardPoint (point: Spec_Ed25519.ext_point) = 
+  match point with 
+  | (px, py, pz, pt) -> Printf.printf "point: %s %s %s %s" (to_string px)  (to_string py) (to_string pz) (to_string pt)
+
+
+let testIsPointOnCurve (point: twisted_edward_point) = 
+  let pointOpt = Some point in 
+  let r = isPointOnCurve pointOpt in 
+    printTwistedEdwardPoint point;  Printf.printf " is on the curve? %b" r                                  
+
+
+let printUint8 (a: FStar_UInt8.t)  = 
+  Printf.printf " %s " (FStar_UInt8.to_string a)
+
+
+let printSeqUInt8 (a:  FStar_UInt8.t FStar_Seq_Base.seq) = 
+  let length = FStar_Seq_Base.length a in 
+    let rec print_inside a counter = 
+      if counter < FStar_Seq_Base.length a then 
+        (
+          printUint8 (FStar_Seq_Base.index a counter);
+          print_inside a (counter + one)
+        )
+      else 
+        Printf.printf "\n" 
+    in print_inside a zero  
+
+let createBuffer (length: nat) (value: FStar_UInt8.t) : FStar_UInt8.t FStar_Seq_Base.seq = 
+  FStar_Seq_Base.create (Prims.parse_int (to_string length)) value  
+
+let bufferEqual (a: FStar_UInt8.t FStar_Seq_Base.seq) (b:FStar_UInt8.t FStar_Seq_Base.seq) = 
+  let rec equal_inside a b counter = 
+    if counter < FStar_Seq_Base.length a then 
+        let flag = FStar_UInt8.eq (FStar_Seq_Base.index a counter) (FStar_Seq_Base.index b counter) in 
+          if (flag = false) then false 
+          else equal_inside a b (counter + one)
+    else 
+      true      
+  in (FStar_Seq_Base.length a = FStar_Seq_Base.length b) && equal_inside a b zero    
+                                  
+
+(* test_vectors for _helper_I2OSP*)
+let test_vector1_helper_i2osp : FStar_UInt8.t Prims.list = 
+        [FStar_UInt8.uint_to_t (Prims.parse_int "160"); 
+          FStar_UInt8.uint_to_t (Prims.parse_int "134");
+          FStar_UInt8.uint_to_t (Prims.parse_int "1");]
+
+let test_vector2_helper_i2osp : FStar_UInt8.t Prims.list = 
+        [
+        FStar_UInt8.uint_to_t (Prims.parse_int "160"); 
+        FStar_UInt8.uint_to_t (Prims.parse_int "134"); 
+        FStar_UInt8.uint_to_t (Prims.parse_int "1");
+        FStar_UInt8.uint_to_t (Prims.parse_int "0");
+        FStar_UInt8.uint_to_t (Prims.parse_int "56");
+        FStar_UInt8.uint_to_t (Prims.parse_int "56");
+        FStar_UInt8.uint_to_t (Prims.parse_int "56");
+        ]
+
+let check_helper_i2osp_1 (vector:FStar_UInt8.t Prims.list) =
+      let buffer = createBuffer (Prims.parse_int "3") (FStar_UInt8.of_string "0") in 
+      let result = _helper_I2OSP (Prims.parse_int "100000") buffer (Prims.parse_int "0") in 
+          printSeqUInt8 result;
+      let expected = (FStar_Seq_Properties.createL vector) in 
+          printSeqUInt8 expected;
+          Printf.printf "Test returned %B \n" (bufferEqual expected result);
+     bufferEqual expected result
+
+let check_helper_i2osp_2 (vector:FStar_UInt8.t Prims.list) =
+      let buffer = createBuffer (Prims.parse_int "7") (FStar_UInt8.of_string "0") in 
+      let result = _helper_I2OSP (Prims.parse_int "15824411865220768") buffer (Prims.parse_int "0") in 
+          printSeqUInt8 result;
+      let expected = (FStar_Seq_Properties.createL vector) in 
+          printSeqUInt8 expected;
+          Printf.printf "Test returned %B \n" (bufferEqual expected result);
+     bufferEqual expected result
+
+let check_i2osp_1 (vector:FStar_UInt8.t Prims.list) = 
+    let result = _I2OSP (Prims.parse_int "15824411865220768") (Prims.parse_int "7") in 
+      printSeqUInt8 result;
+    let expected = (FStar_Seq_Properties.createL vector) in
+      printSeqUInt8 expected;
+      Printf.printf "Test returned %B \n" (bufferEqual expected result);
+    bufferEqual expected result
+
+
+let check_osp2i_1 (vector:FStar_UInt8.t Prims.list) = 
+    let vector = (FStar_Seq_Properties.createL vector) in
+    let result = _OS2IP vector in 
+      Printf.printf "The number %s \n" (to_string result);
+      Printf.printf "Test returned %B \n" ((Prims.parse_int "15824411865220768") = result);
+    ((Prims.parse_int "15824411865220768") = result)  
+
+
+let _ = 
+  check_helper_i2osp_1 test_vector1_helper_i2osp;
+  check_helper_i2osp_2 test_vector2_helper_i2osp;
+  check_i2osp_1 test_vector2_helper_i2osp;
+  check_osp2i_1 test_vector2_helper_i2osp                                 
