VRF/Spec.VRF.fst
@@ -1,5 +1,6 @@
 module Spec.VRF
 
+
 open FStar.UInt32
 open FStar.UInt8
 open FStar.Seq
@@ -7,214 +8,248 @@ open FStar.Option
 
 open FStar.Mul
 open FStar.Seq
-open FStar.UInt8
+open FStar.UInt
+
+
 open FStar.Endianness
-open Spec.Lib
-open Spec.Curve25519.Lemmas
 open Spec.Curve25519
+open Spec.Ed25519
+(*)
 open Spec.SHA2_256
+*)
 
-
+#set-options "--max_fuel 0 --initial_fuel 0"
 
 let bytes =  seq FStar.UInt8.t
 let key = lbytes 32
-let order = 2
-let field = 100000000000
+let field = prime
 
 let n = 32
 
-let positive_point_const = Seq.create 1 2uy
-let negative_point_const = Seq.create 1 3uy
 
-assume val scalarMultiplication: point:serialized_point -> k: scalar -> Tot serialized_point
-assume val scalarAddition: p: serialized_point -> q: serialized_point -> Tot serialized_point
-assume val isPointOnCurve: p: option serialized_point -> Tot(bool)
-assume val deserializePoint: serialized_point -> Tot (tuple2 int int) (* I am just a wrapper *)
+let d : elem = 37095705934669439343138083508754565189542113879843219016388785533085940283555
+type twisted_edward_point = ext_point
 
-(* PRIME NUMBER CASE! *)
+val scalarMultiplication : point : twisted_edward_point -> k: bytes -> Tot twisted_edward_point
+let scalarMultiplication point k = 
+	Spec.Ed25519.point_mul k point
 
-assume val _OS2ECP : bytes -> Tot(serialized_point)
+val scalarAddition : p : twisted_edward_point -> q: twisted_edward_point -> Tot twisted_edward_point
+let scalarAddition p q = 
+	Spec.Ed25519.point_add p q 
+
+val isPointOnCurve: point : option twisted_edward_point -> Tot bool
+let isPointOnCurve point =
+	if isNone point then false else
+	let point = get point in 
+	let px, py, pz, pt = point in 
+	let x2 = fmul px px in 
+	let y2 = fmul py py in 
+	let left = fsub x2 y2 in 
+	let z2 = fmul pz pz in 
+	let t2 = fmul pt pt in 
+	let dt2 = fmul d t2 in 
+	let right = fadd z2 dt2 in 
+	(left = right)
+
+
+val serializePoint : point: twisted_edward_point -> Tot bytes
+let serializePoint point = point_compress point
+
+val deserializePoint : b: bytes{Seq.length b = 32} -> Tot (option twisted_edward_point)
+let deserializePoint b = point_decompress b
+
+val _OS2ECP : point: bytes{Seq.length point = 32} -> Tot(option twisted_edward_point)
+let _OS2ECP point = deserializePoint point
+
+val _ECP2OS : gamma: twisted_edward_point -> Tot(r: bytes {Seq.length r = 32})
+let _ECP2OS gamma = serializePoint gamma
 
 val nat_to_uint8: x: int {x < 256} -> Tot(FStar.UInt8.t)
-let nat_to_uint8 x = FStar.UInt8.uint_to_t x
+let nat_to_uint8 x = FStar.UInt8.uint_to_t (to_uint_t 8 x)
 
 val uint8_to_int : x: FStar.UInt8.t -> Tot(int)
 let uint8_to_int x = FStar.UInt8.v x
 
-val _helper_I2OSP: value: int -> n: nat -> counter : nat {counter <= n} -> s: bytes -> Tot (r: bytes {Seq.length r = Seq.length s})
-let rec _helper_I2OSP value n counter s = 
-    let mask = 256 in 
-    let r = value %256 in 
-    let r = nat_to_uint8 r in 
-    let s = upd s counter r in 
-    let number = value / mask  in 
-        if (counter +1 <=n) then 
-            _helper_I2OSP value n (counter +1) s
-        else s
+val _helper_I2OSP: value: nat -> s: bytes -> counter : nat {counter < Seq.length s} -> 
+		Tot (r: bytes {Seq.length r = Seq.length s})(decreases (Seq.length s - counter))
+let rec _helper_I2OSP value s counter  = 
+	let mask = 256 in 
+	let r = value % mask in 
+	let r = nat_to_uint8 r in 
+	let s = upd s counter r in 
+	let number = value / mask  in (*changed *)
+		if (counter +1 <Seq.length s) then 
+			_helper_I2OSP number s (counter +1)
+		else s
 
-val _I2OSP: value1: int -> n: int{n > 0} -> Tot(r: bytes{Seq.length r = n})
-let _I2OSP value1 n = 
-    if (pow2 n <= value1) then Seq.create n 0uy
-    else 
-        let s = Seq.create n 0uy in 
-         (_helper_I2OSP value1 n 0 s)
+val _I2OSP: value: nat -> n: int{n > 0} -> Tot(r: bytes{Seq.length r = n})
+let _I2OSP value n = 
+	if (pow2 (n * 8)  <= value) then Seq.create n 0uy (* changed*)
+	else 
+		let s = Seq.create n 0uy in 
+		 (_helper_I2OSP value s 0)
 
-val _helper_OS2IP: s: bytes  -> counter: nat {counter < Seq.length s} -> number: int -> Tot (int)
+val _helper_OS2IP: s: bytes  -> counter: nat {counter < Seq.length s} -> number: nat -> 
+	Tot (nat)(decreases (Seq.length s - counter))
+
 let rec _helper_OS2IP s counter number = 
-    let temp = Seq.index s counter in 
-    let temp = uint8_to_int temp in 
-    let number = number + (op_Multiply (pow2 8*counter) temp) in 
-    if (counter + 1 = Seq.length s) then number else _helper_OS2IP s (counter+1) number
+	let temp = Seq.index s counter in 
+	let temp = uint8_to_int temp in 
+	let counter_mult = pow2 (8 * counter) in 
+	let number = number + (op_Multiply counter_mult temp) in 
+	if (counter + 1 = Seq.length s) then 
+		number 
+	else _helper_OS2IP s (counter+1) number
 
 val _OS2IP: s: bytes{Seq.length s > 0} -> nat
 
 let _OS2IP s = 
-    _helper_OS2IP s 0 0
+	_helper_OS2IP s 0 0
 
 val seqConcat : s1: seq 'a -> s2: seq 'a -> 
-            Tot(r:seq 'a{Seq.length    r = Seq.length s1 + Seq.length s2})
+			Tot(r:seq 'a{Seq.length	r = Seq.length s1 + Seq.length s2})
 
 let seqConcat s1 s2 = 
-    FStar.Seq.append s1 s2     
+	FStar.Seq.append s1 s2 	
 
-val _ECP2OS : gamma: serialized_point -> Tot(r: bytes {Seq.length r = (op_Multiply 2 n) + 1})
-let _ECP2OS gamma = 
-    let x,y = deserializePoint gamma in 
-    let y' = y / 2 in 
-    let x = _I2OSP x (op_Multiply 2 n) in 
-    if y' = 0 then 
-        seqConcat positive_point_const x
-    else
-        seqConcat negative_point_const x    
-
-val hash: input: bytes{Seq.length input < pow2 61} -> Tot(bytes)    
+val hash: input: bytes{Seq.length input < Spec.SHA2_256.max_input_len_8} -> 
+		Tot(r: bytes{Seq.length r = Spec.SHA2_256.size_hash})	
 let hash input = 
-    Spec.SHA2_256.hash input
+	Spec.SHA2_256.hash input
 
-val _helper_ECVRF_hash_to_curve : 
-    ctr : nat -> input: bytes{Seq.length input < pow2 61 - (op_Multiply 2 n) - 5 } -> pk: bytes -> Tot(r: option serialized_point{isPointOnCurve r})(decreases(field - ctr))
-
-let rec _helper_ECVRF_hash_to_curve ctr input pk = 
-    let _CTR = _I2OSP ctr 4 in 
-    let toHash = seqConcat input pk in 
-    let toHash = seqConcat toHash _CTR in 
-    let hash = hash toHash in 
-    let possible_point = seqConcat positive_point_const hash in 
-        if isPointOnCurve (Some possible_point) then Some possible_point 
-        else
-            let possible_point    = seqConcat negative_point_const hash in 
-                if isPointOnCurve (Some possible_point) then Some possible_point 
-                else 
-                    if (ctr +1) < field 
-                        then _helper_ECVRF_hash_to_curve (ctr+1) input pk 
-                    else None    
-
-
-val _ECVRF_hash_to_curve: input: bytes{Seq.length input < pow2 61 - (op_Multiply 2 n) - 5 } -> 
-            public_key: (serialized_point) -> Tot(option serialized_point)            
-
-let _ECVRF_hash_to_curve input public_key = 
-    let ctr = 0 in 
-    let pk = _ECP2OS public_key in 
-    let point = _helper_ECVRF_hash_to_curve ctr input pk in point
-
-assume val random:     max: nat -> Tot(random : nat {random <= max})    
-
-val randBytes: max: nat -> Tot(bytes) 
-let randBytes max = 
-    let rand = random max in _I2OSP rand 32 (* in octets = log_2 field / 8  *)
-
-val _ECVRF_hash_points : generator: serialized_point -> h:  serialized_point -> 
-            public_key: serialized_point -> gamma : serialized_point -> 
-            gk : serialized_point -> hk : serialized_point -> 
-            Tot(int)
-
-let _ECVRF_hash_points generator h public_key gamma gk hk = 
-    let p = _ECP2OS generator in (*2n +1 = 33 *)
-    let p = seqConcat p (_ECP2OS h) in (* 66  *)
-    let p = seqConcat p (_ECP2OS public_key) (* 99 *) in 
-    let p = seqConcat p (_ECP2OS gamma)  (* still less than 2pow 61 *)in 
-    let p = seqConcat p (_ECP2OS gk) in 
-    let p = seqConcat p (_ECP2OS hk) in 
-    let h' = hash p in 
-    let h = fst (FStar.Seq.split h' n) in 
-    _OS2IP h
-
-val _ECVRF_prove: input: bytes {Seq.length input < pow2 61 - (op_Multiply 2 n) - 5 } ->  public_key: serialized_point -> 
-            private_key : bytes (* private key in this scope is a mupliplier of the generator *)
-            -> generator : serialized_point->  
-            Tot(proof: option bytes {Some?proof ==> Seq.length (Some?.v proof) = (op_Multiply 5 n) + 1})
-            (*Tot(proof: option bytes{Seq.length proof = 5 * n + 1})  *)
-
-let _ECVRF_prove input public_key private_key generator = 
-    let h = _ECVRF_hash_to_curve input public_key in 
-        if isNone h then None (* trying to convert the hash to point, 
-        if it was not possible returns None *)
-        else 
-            let h = get h in 
-    let gamma = scalarMultiplication h private_key in 
-    let k =  randBytes field in  (* random in sequence  *)
-        let gk = scalarMultiplication generator k in  (* k< (2^8)^32 = 2^(8*32) = 2^(2^3 * 2^ 5 = 256) *) (* *)
-        let hk = scalarMultiplication h k in 
-    let c = _ECVRF_hash_points generator h public_key gamma gk hk in (*int*)
-            let cq = op_Multiply c field in  (*int*)
-            let cqmodq = cq % field in 
-            let k_ = _OS2IP k in (* random was generated in the seq -> cast to nat *)
-    let s = k_ - cqmodq (* int *) in 
-            let fst = _ECP2OS gamma in 
-            let snd = _I2OSP c n in (* Seq length snd = n*)
-            let thd = _I2OSP s ( op_Multiply 2 n) (* Seq.length thr = 2n *) in 
-    let pi = seqConcat fst (seqConcat snd thd) in Some pi
-
-val _ECVRF_rec : counter: nat -> counter_local: nat{counter_local < counter} -> 
-                s: seq 'a {Seq.length s > counter} -> r_temp : seq 'a ->
-                Tot(r: seq 'a)(decreases (counter - counter_local))
-
-let rec _ECVRF_rec counter counter_local s r_temp =
-    let r_temp = seqConcat r_temp (Seq.create 1 (Seq.index s counter_local)) in 
-    if (counter_local + 1) < counter 
-        then _ECVRF_rec counter (counter_local +1) s r_temp
-    else 
-        r_temp
-
-val _ECVRF_proof2hash: pi: bytes{Seq.length pi = op_Multiply 5 n + 1} -> Tot(hash: bytes)
-let _ECVRF_proof2hash pi = 
-    let r_temp = Seq.createEmpty in 
-     _ECVRF_rec (op_Multiply 2 n + 1) 2 pi r_temp
+#set-options "--initial_ifuel 1 --max_ifuel 1 --initial_fuel 0 --max_fuel 0 --z3rlimit 30"
 
 
 val _ECVRF_decode_proof: 
-        pi: bytes {Seq.length pi = op_Multiply 5 n + 1} -> 
-        Tot(tuple3 (option serialized_point) bytes bytes) (* due to the fact that
-         we do point multiplication using seq of bytes, 
-        the operation to cast the value to int and to sequence 
-        back is decided to be needless*)
+		pi: bytes {Seq.length pi = op_Multiply 4 n} -> 
+		Tot(tuple3 (option twisted_edward_point) (c:bytes{Seq.length c = n}) (s:bytes {Seq.length s = (op_Multiply 2 n)}))
+		 (* due to the fact that
+		 we do point multiplication using seq of bytes, 
+		the operation to cast the value to int and to sequence 
+		back is decided to be needless*)
 
 let _ECVRF_decode_proof pi = 
-    let gamma, cs = Seq.split pi ((op_Multiply 2 n)+1) in 
-    let c, s = Seq.split cs n in 
-    (Some(_OS2ECP gamma), c, s)
+	let gamma, cs = Seq.split pi n in 
+		assert(Seq.length gamma = n);
+		assert(Seq.length cs = op_Multiply 3 n);
+	let c, s = Seq.split cs n in 
+		assert(Seq.length c = n);
+		assert(Seq.length s = op_Multiply 2 n);
+	let point = _OS2ECP gamma in 
+	(point, c, s)
+
+#reset-options
 
 
-val _ECVRF_verify : generator: serialized_point ->  public_key : serialized_point ->
-        pi: bytes {Seq.length pi = op_Multiply 5 n +1} -> 
-        input : bytes -> 
-        Tot(bool)
+val _helper_ECVRF_hash_to_curve : 
+	ctr : nat{ctr < field} ->counter_length:nat{counter_length > 0} ->  
+	pk: bytes{Seq.length pk = 32} ->
+	input: bytes{Seq.length input < Spec.SHA2_256.max_input_len_8 - 32 - counter_length } ->
+	Tot(r: option twisted_edward_point {Some?r ==> isPointOnCurve r}) 
+	(decreases(field - ctr)) 
+
+let rec _helper_ECVRF_hash_to_curve ctr counter_length pk input = 
+	let _CTR = _I2OSP ctr counter_length in 
+	let toHash = seqConcat input pk in 
+	let toHash = seqConcat toHash _CTR in (* point nonce *)
+	let hash = hash toHash in
+	(*let possible_point = seqConcat positive_point_const hash in*) (* this one was deleted becauce of decompression func *) 
+	(*let possible_point = _OS2ECP possible_point in *)
+	let possible_point = _OS2ECP hash in 
+	if isNone possible_point then None else
+		if isPointOnCurve possible_point then possible_point
+		else
+			if (ctr +1) < field
+				then (
+					assert((ctr+1) <field);
+					_helper_ECVRF_hash_to_curve (ctr+1) counter_length pk input)
+			else None	
+
+val _ECVRF_hash_to_curve: input: bytes{Seq.length input < Spec.SHA2_256.max_input_len_8 - 36 } -> 
+			public_key: (twisted_edward_point) -> Tot(option twisted_edward_point)			
+
+let _ECVRF_hash_to_curve input public_key = 
+	let ctr = 0 in 
+	let pk = _ECP2OS public_key in 
+	let point = _helper_ECVRF_hash_to_curve ctr 4 pk input in point
+
+assume val random: 	max: nat -> Tot(random : nat {random > 0 /\ random < max})	
+
+val randBytes: max: nat -> Tot(r:bytes{Seq.length r = 32})
+let randBytes max = 
+	let rand = random max in _I2OSP rand 32 (* in octets = log_2 field / 8  *)
+
+val _ECVRF_hash_points : generator: twisted_edward_point -> h:  twisted_edward_point -> 
+			public_key: twisted_edward_point -> gamma : twisted_edward_point -> 
+			gk : twisted_edward_point -> hk : twisted_edward_point -> 
+			Tot(nat)
+
+let _ECVRF_hash_points generator h public_key gamma gk hk = 
+	let p = _ECP2OS generator in (*32 *)
+	let p = seqConcat p (_ECP2OS h) in (* 64  *)
+	let p = seqConcat p (_ECP2OS public_key) (* 32*3 *) in 
+	let p = seqConcat p (_ECP2OS gamma)  (* still less than 2pow 61 *)in 
+	let p = seqConcat p (_ECP2OS gk) in 
+	let p = seqConcat p (_ECP2OS hk) in 
+	let h' = hash p in 
+	let h = fst (FStar.Seq.split h' n) in 
+	_OS2IP h
+
+val _ECVRF_prove: input: bytes {Seq.length input < Spec.SHA2_256.max_input_len_8 - 36 } ->  public_key: twisted_edward_point -> 
+			private_key : bytes (* private key in this scope is a mupliplier of the generator *)
+			-> generator : twisted_edward_point->  
+			Tot(proof: option bytes {Some?proof ==> Seq.length (Some?.v proof) = op_Multiply 4 n})
+			(*Tot(proof: option bytes{Seq.length proof = 5 * n + 1})  *)
+
+let _ECVRF_prove input public_key private_key generator = 
+	let h = _ECVRF_hash_to_curve input public_key in 
+		if isNone h then None (* trying to convert the hash to point, if it was not possible returns None *)
+		else 
+			let h = get h in 
+	let gamma = scalarMultiplication h private_key in 
+	let k_ = random field in 
+	let k =  _I2OSP k_ 32 in  (* random in sequence  *)
+		let gk = scalarMultiplication generator k in  (* k< (2^8)^32 = 2^(8*32) = 2^(2^3 * 2^ 5 = 256) *) (* *)
+		let hk = scalarMultiplication h k in 
+	let c = _ECVRF_hash_points generator h public_key gamma gk hk in (*int*)
+			let cq = op_Multiply c field in  (*int*)
+			let cqmodq = cq % field in 
+			assert(cqmodq < field);
+			assert(k_ <field); 
+			assert(k_ + field > field); (* I assume that the operations are done in the field. *)
+	let k_ = k_ + field in 		
+			(* random was generated in the seq -> cast to nat *)
+	let s = k_ - cqmodq (* int *) in (*cqmodq is < field *)
+	assert (s > 0);
+			let fst = _ECP2OS gamma in (*32*)
+			let snd = _I2OSP c n in (* Seq length snd = n*)
+			let thd = _I2OSP s ( op_Multiply 2 n) (* Seq.length thr = 2n *) in 
+	let pi = seqConcat fst (seqConcat snd thd) in Some pi
+
+
+val _ECVRF_proof2hash: pi: bytes{Seq.length pi = op_Multiply 4 n } -> Tot(hash: bytes{Seq.length hash = n})
+let _ECVRF_proof2hash pi = fst( Seq.split pi n)
+
+val _ECVRF_verify : generator: twisted_edward_point ->  public_key : twisted_edward_point ->
+		pi: bytes {Seq.length pi = op_Multiply 4 n } -> 
+		input : bytes{Seq.length input < Spec.SHA2_256.max_input_len_8 - 36 } -> 
+		Tot(bool)
 
 let _ECVRF_verify generator public_key pi input = 
-    let gamma, c, s = _ECVRF_decode_proof pi in 
-    if not(isPointOnCurve gamma) then false else
-    if isNone gamma then false
-        else let gamma = get gamma in 
-    let pkc = scalarMultiplication public_key c in 
-    let gs = scalarMultiplication generator s in 
-    let u  = scalarAddition pkc gs in 
-    let h = _ECVRF_hash_to_curve input public_key in 
-        if isNone h then false
-    else 
-    let h = get h in 
-    let gammac = scalarMultiplication gamma c in 
-    let hs = scalarMultiplication h s in 
-    let v = scalarAddition gammac hs in 
-    let c_prime = _ECVRF_hash_points generator h public_key gamma u v in 
-    (_OS2IP c) = c_prime
+	let gamma, c, s = _ECVRF_decode_proof pi in 
+	if not(isPointOnCurve gamma) then false else
+	if isNone gamma then false
+		else let gamma = get gamma in 
+	let pkc = scalarMultiplication public_key c in 
+	let gs = scalarMultiplication generator s in 
+	let u  = scalarAddition pkc gs in 
+	let h = _ECVRF_hash_to_curve input public_key in 
+		if isNone h then false
+	else 
+	let h = get h in 
+	let gammac = scalarMultiplication gamma c in 
+	let hs = scalarMultiplication h s in 
+	let v = scalarAddition gammac hs in 
+	let c_prime = _ECVRF_hash_points generator h public_key gamma u v in 
+	(_OS2IP c) = c_prime
